dijkstra/verif_dijkstra1.v
@@ -26,6 +26,8 @@ Section DijkstraProof.
 
   Context {size: Z}.
   Context {inf: Z}.
+  Context {V_EqDec : EquivDec.EqDec V eq}.
+  Context {E_EqDec : EquivDec.EqDec E eq}.
 
   Definition dijk_setup_loop_inv g sh src dist prev v_pq arr addresses :=
     EX i : Z,
@@ -57,7 +59,7 @@ Section DijkstraProof.
         DijkGraph sh CompSpecs g (pointer_val_val arr) size addresses;
         free_tok (pointer_val_val v_pq) (sizeof tint * size)).
   
-  Definition dijk_forloop_inv (g: @DijkGG size inf) sh src
+  Definition dijk_forloop_inv (g: @DijkGG size inf _ _) sh src
              dist_ptr prev_ptr priq_ptr graph_ptr addresses :=
     EX prev : list V,
     EX priq : list V,
@@ -112,7 +114,7 @@ Section DijkstraProof.
              DijkGraph sh CompSpecs g (pointer_val_val graph_ptr) size addresses;
              free_tok (pointer_val_val priq_ptr) (sizeof tint * size)).
   
-  Definition dijk_forloop_break_inv (g: @DijkGG size inf) sh
+  Definition dijk_forloop_break_inv (g: @DijkGG size inf _ _) sh
                                     src dist_ptr prev_ptr priq_ptr
                                     graph_ptr addresses :=
     EX prev: list V,
@@ -140,7 +142,7 @@ Section DijkstraProof.
              DijkGraph sh CompSpecs g (pointer_val_val graph_ptr) size addresses;
              free_tok (pointer_val_val priq_ptr) (sizeof tint * size)).
   
-  Definition dijk_inner_forloop_inv (g: @DijkGG size inf) sh
+  Definition dijk_inner_forloop_inv (g: @DijkGG size inf _ _) sh
              src (priq dist prev : list Z)
              dist_ptr prev_ptr priq_ptr graph_ptr addresses :=
     EX i : Z,
@@ -242,21 +244,21 @@ Section DijkstraProof.
              free_tok (pointer_val_val priq_ptr) (sizeof tint * size)).
   
 
-  Lemma body_getCell: semax_body Vprog (@Gprog size inf) f_getCell (@getCell_spec size inf).
+  Lemma body_getCell: semax_body Vprog (@Gprog size inf _ _) f_getCell (@getCell_spec size inf _ _).
   Proof.
     start_function.
     unfold DijkGraph.
     rewrite (SpaceAdjMatGraph_unfold _ id _ _ addresses u); trivial.
 
-    assert (Zlength (map Int.repr (Znth u (@graph_to_mat size g id))) = size). {
+    assert (Zlength (map Int.repr (Znth u (@graph_to_mat size _ _ g id))) = size). {
       unfold graph_to_mat, vert_to_list.
       rewrite Znth_map; repeat rewrite Zlength_map.
       all: rewrite nat_inc_list_Zlength; lia.
     }
 
-    assert (0 <= i < Zlength (map Int.repr (Znth u (@graph_to_mat size g id)))) by lia.
+    assert (0 <= i < Zlength (map Int.repr (Znth u (@graph_to_mat size _ _ g id)))) by lia.
 
-    assert (0 <= i < Zlength (Znth u (@graph_to_mat size g id))). {
+    assert (0 <= i < Zlength (Znth u (@graph_to_mat size _ _ g id))). {
       rewrite Zlength_map in H1. lia.
     }
     
@@ -271,7 +273,7 @@ Section DijkstraProof.
 
   (* DIJKSTRA PROOF BEGINS *)
 
-  Lemma body_dijkstra: semax_body Vprog (@Gprog size inf) f_dijkstra (@dijkstra_spec size inf).
+  Lemma body_dijkstra: semax_body Vprog (@Gprog size inf _ _) f_dijkstra (@dijkstra_spec size inf _ _).
   Proof.
     start_function.
     pose proof (size_further_restricted g).
@@ -389,7 +391,7 @@ Section DijkstraProof.
         assert (H_inrange_priq_trans:
                   forall priq,
                     @inrange_priq inf priq ->
-                    priq_arr_utils.inrange_priq inf priq). {
+                    @priq_arr_utils.inrange_priq inf priq). {
           intros.
           red in H11 |- *.
           rewrite Forall_forall in H11 |- *.
@@ -408,8 +410,8 @@ Section DijkstraProof.
         forward_if. (* checking if it's time to break *)
         * (* No, don't break. *)
           rename H11 into Htemp.
-          assert (isEmpty priq inf = Vzero). {
-            destruct (isEmptyTwoCases priq inf);
+          assert (@isEmpty inf priq = Vzero). {
+            destruct (@isEmptyTwoCases inf priq);
               rewrite H11 in Htemp; simpl in Htemp;
                 now inversion Htemp.
           }
@@ -617,7 +619,7 @@ Section DijkstraProof.
             rename H30 into H26.
 
             forward_call (sh, g, graph_ptr, addresses, u, i).
-            remember (Znth i (Znth u (@graph_to_mat size g id))) as cost.
+            remember (Znth i (Znth u (@graph_to_mat size _ _ g id))) as cost.
 
             assert (H_i_valid: vvalid g i). {
               apply (vvalid_meaning g); trivial.
@@ -636,7 +638,8 @@ Section DijkstraProof.
                  rewrite Int.signed_repr in Htemp; trivial.
                  rewrite <- H28 in Htemp.
                  apply Zlt_not_le in Htemp.
-                 apply Htemp; reflexivity. (* lemma-fy *)
+                 apply Htemp.
+                 reflexivity.
                }
                clear Htemp.
                assert (H_ui_valid: evalid g (u,i)). {
@@ -670,7 +673,6 @@ Section DijkstraProof.
                   (* We know that we are definitely
                    going to make edits in the arrays:
                    we have found a better path to i, via u *)
-                  
                   rename H28 into Htemp.
                   assert (H28: 0 <= Znth u dist' < inf) by lia.
                   clear Htemp.
@@ -911,14 +913,14 @@ Section DijkstraProof.
             
         * (* After breaking from the while loop,
            prove break's postcondition *)
-          assert (isEmpty priq inf = Vone). {
-            destruct (isEmptyTwoCases priq inf); trivial.
+          assert (@isEmpty inf priq = Vone). {
+            destruct (@isEmptyTwoCases inf priq); trivial.
             rewrite H12 in H11; simpl in H11; now inversion H11.
           }
           clear H11.
           forward. Exists prev priq dist popped.
           entailer!.
-          pose proof (isEmptyMeansInf priq inf).
+          pose proof (@isEmptyMeansInf inf priq).
           rewrite H25 in H12.
           rewrite Forall_forall in H12 |- *.
           intros. specialize (H12 _ H26). lia.
