prim/MatrixUGraph.v
@@ -41,9 +41,9 @@ Qed.
 
 Section MATRIXUGRAPH.
 
-  Context {size: Z} {inf: Z}.
-
-  Instance Z_EqDec : EqDec Z eq. Proof. hnf. intros. apply Z.eq_dec. Defined.
+Context {size: Z} {inf: Z}.
+Context {V_EqDec : EquivDec.EqDec V eq}. 
+Context {E_EqDec : EquivDec.EqDec E eq}. 
 
 Class AdjMatUSoundness (g: AdjMatLG) := {
   sadjmat: SoundAdjMat (size:=size) (inf:=inf) g;
@@ -56,7 +56,7 @@ Definition MatrixUGraph := (GeneralGraph V E DV DE DG (fun g => AdjMatUSoundness
 
 Definition sound_MatrixUGraph (g: MatrixUGraph) := (@sound_gg _ _ _ _ _ _ _ _ g).
 Definition sound_adjMatGraph (g: MatrixUGraph) := (@sadjmat g (sound_MatrixUGraph g)).
-Definition finGraph (g: MatrixUGraph) := (@fin _ _ g (sound_adjMatGraph g)).
+Definition finGraph (g: MatrixUGraph) := (@fin _ _ _ _ g (sound_adjMatGraph g)).
 
 Instance Finite_MatrixUPGraph (g: MatrixUGraph): FiniteGraph g.
 Proof. apply (finGraph g). Qed.
@@ -67,25 +67,25 @@ Coercion MatrixUGraph_AdjMatGG: MatrixUGraph >-> AdjMatGG.
 
 (*still nitty-gritty issues with the coercion*)
 Definition size_representable (g: MatrixUGraph) :=
-  @sr _ _ g (sound_adjMatGraph g).
+  @sr _ _ _ _ g (sound_adjMatGraph g).
 
 Definition inf_representable (g: MatrixUGraph) :=
-  @ir _ _ g (sound_adjMatGraph g).
+  @ir _ _ _ _ g (sound_adjMatGraph g).
 
 Definition vvalid_meaning (g: MatrixUGraph) :=
-  @vm _ _ g (sound_adjMatGraph g).
+  @vm _ _ _ _ g (sound_adjMatGraph g).
 
 Definition evalid_meaning (g: MatrixUGraph) :=
-  @em _ _ g (sound_adjMatGraph g).
+  @em _ _ _ _ g (sound_adjMatGraph g).
 
 Definition invalid_edge_weight (g: MatrixUGraph) :=
-  @iew _ _ g (sound_adjMatGraph g).
+  @iew _ _ _ _ g (sound_adjMatGraph g).
 
 Definition src_fst (g: MatrixUGraph) :=
-  @esf _ _ g (sound_adjMatGraph g).
+  @esf _ _ _ _ g (sound_adjMatGraph g).
 
 Definition dst_snd (g: MatrixUGraph) :=
-  @eds _ _ g (sound_adjMatGraph g).
+  @eds _ _ _ _ g (sound_adjMatGraph g).
 
 Definition evalid_strong_evalid (g: MatrixUGraph) :=
   @ese g (sound_MatrixUGraph g).
@@ -860,19 +860,19 @@ assert (find (a :: l') x 0 <= find (a :: l') y 0 <-> find (a :: l) x 0 <= find (
 right; auto. right; auto.
 apply NoDup_cons_2 in H3.
 simpl in H8.
-destruct (prod_eqdec Z_EqDec Z_EqDec a x). hnf in e. subst x. contradiction.
-destruct (prod_eqdec Z_EqDec Z_EqDec a y). hnf in e. subst y. contradiction.
+destruct (E_EqDec a x). hnf in e. subst x. contradiction.
+destruct (E_EqDec a y). hnf in e. subst y. contradiction.
 replace 1 with (1+0) in H8 by lia. repeat rewrite find_accum_add1 in H8.
 split; intros. lia. lia.
 ******
 unfold complement, equiv in c.
 assert (find (e :: l') e 0 <= find (e :: l') a 0 <-> find (a :: l) e 0 <= find (a :: l) a 0). apply H5.
 left; auto. auto. simpl in H6.
-destruct (prod_eqdec Z_EqDec Z_EqDec e e). 2: { unfold complement, equiv in c0; contradiction. }
-destruct (prod_eqdec Z_EqDec Z_EqDec a a). 2: { unfold complement, equiv in c0; contradiction. }
+destruct (E_EqDec e e). 2: { unfold complement, equiv in c0; contradiction. }
+destruct (E_EqDec a a). 2: { unfold complement, equiv in c0; contradiction. }
 clear e0 e1.
-destruct (prod_eqdec Z_EqDec Z_EqDec e a). hnf in e0; contradiction.
-destruct (prod_eqdec Z_EqDec Z_EqDec a e). hnf in e0; symmetry in e0; contradiction.
+destruct (E_EqDec e a). hnf in e0; contradiction.
+destruct (E_EqDec a e). hnf in e0; symmetry in e0; contradiction.
 clear c0 c1.
 assert (0 <= find l' a 1). { apply (Z.le_trans 0 1). lia. apply find_lbound. }
 apply H6 in H7. assert (1 <= 0). { apply (Z.le_trans 1 (find l e 1)). apply find_lbound. auto. }
@@ -881,8 +881,8 @@ lia.
 left. apply H1. split. auto. split. unfold incl; intros. assert (In a0 (a::l)). apply H4; auto.
 destruct H7. subst a0. contradiction. auto.
 intros. assert (find l' x 0 <= find l' y 0 <-> find (a :: l) x 0 <= find (a :: l) y 0). apply H5; auto.
-simpl in H8. destruct (prod_eqdec Z_EqDec Z_EqDec a x). hnf in e. subst x. contradiction.
-destruct (prod_eqdec Z_EqDec Z_EqDec a y). hnf in e. subst y. contradiction.
+simpl in H8. destruct (E_EqDec a x). hnf in e. subst x. contradiction.
+destruct (E_EqDec a y). hnf in e. subst y. contradiction.
 replace 1 with (1+0) in H8 by lia. do 2 rewrite find_accum_add1 in H8.
 split; intros. apply H8 in H9. lia.
 apply H8. lia.
@@ -894,8 +894,8 @@ split. auto. split. unfold incl; intros. right. apply H4. auto.
 intros.
 assert (find l' x 0 <= find l' y 0 <-> find l x 0 <= find l y 0). apply H5; auto.
 simpl.
-destruct (prod_eqdec Z_EqDec Z_EqDec a x). hnf in e; subst x. apply H4 in H6; contradiction.
-destruct (prod_eqdec Z_EqDec Z_EqDec a y). hnf in e; subst y. apply H4 in H7; contradiction.
+destruct (E_EqDec a x). hnf in e; subst x. apply H4 in H6; contradiction.
+destruct (E_EqDec a y). hnf in e; subst y. apply H4 in H7; contradiction.
 replace 1 with (1+0) by lia. do 2 rewrite (find_accum_add1).
 split; intros. apply H8 in H9. lia. lia.
 ****
@@ -905,16 +905,16 @@ split. apply NoDup_cons; auto.
 split. unfold incl; intros. destruct H7. subst a0. left; auto.
 right. apply H5. auto.
 intros. destruct H7.
-subst x. simpl. destruct (prod_eqdec Z_EqDec Z_EqDec a a). 2: { unfold complement, equiv in c; contradiction. }
-destruct (prod_eqdec Z_EqDec Z_EqDec a y). lia. split; intros. apply (Z.le_trans 0 1). lia. apply find_lbound. apply (Z.le_trans 0 1). lia. apply find_lbound.
+subst x. simpl. destruct (E_EqDec a a). 2: { unfold complement, equiv in c; contradiction. }
+destruct (E_EqDec a y). lia. split; intros. apply (Z.le_trans 0 1). lia. apply find_lbound. apply (Z.le_trans 0 1). lia. apply find_lbound.
 destruct H8. subst y. simpl.
-destruct (prod_eqdec Z_EqDec Z_EqDec a a). 2: { unfold complement, equiv in c; contradiction. }
-destruct (prod_eqdec Z_EqDec Z_EqDec a x). lia. split; intros.
+destruct (E_EqDec a a). 2: { unfold complement, equiv in c; contradiction. }
+destruct (E_EqDec a x). lia. split; intros.
 assert (1 <= 0). apply (Z.le_trans 1 (find l' x 1)). apply find_lbound. lia. lia.
 assert (1 <= 0). apply (Z.le_trans 1 (find l x 1)). apply find_lbound. lia. lia.
 assert (find l' x 0 <= find l' y 0 <-> find l x 0 <= find l y 0). apply H6; auto. simpl.
-destruct (prod_eqdec Z_EqDec Z_EqDec a x). hnf in e; subst x; contradiction.
-destruct (prod_eqdec Z_EqDec Z_EqDec a y). hnf in e; subst y; contradiction.
+destruct (E_EqDec a x). hnf in e; subst x; contradiction.
+destruct (E_EqDec a y). hnf in e; subst y; contradiction.
 replace 1 with (1+0) by lia. repeat rewrite find_accum_add1.
 split; intros; lia.
 Qed.
@@ -949,13 +949,13 @@ apply IHlsorted. 2: { unfold not; intros. apply Ha. right; auto. }
 intros. split; intros.
 apply H2. right; auto. right; auto.
 apply NoDup_cons_2 in Hsorted_NoDup.
-simpl. destruct (prod_eqdec Z_EqDec Z_EqDec a0 a1). hnf in e; subst a0; contradiction.
-destruct (prod_eqdec Z_EqDec Z_EqDec a0 b). hnf in e; subst a0; contradiction.
+simpl. destruct (E_EqDec a0 a1). hnf in e; subst a0; contradiction.
+destruct (E_EqDec a0 b). hnf in e; subst a0; contradiction.
 replace 1 with (1+0) by lia. do 2 rewrite find_accum_add1. lia.
 apply H2 in H4. 2: right; auto. 2: right; auto.
 simpl in H4. apply NoDup_cons_2 in Hsorted_NoDup.
-destruct (prod_eqdec Z_EqDec Z_EqDec a0 a1). hnf in e; subst a0; contradiction.
-destruct (prod_eqdec Z_EqDec Z_EqDec a0 b). hnf in e; subst a0; contradiction.
+destruct (E_EqDec a0 a1). hnf in e; subst a0; contradiction.
+destruct (E_EqDec a0 b). hnf in e; subst a0; contradiction.
 replace 1 with (1+0) in H4 by lia. do 2 rewrite find_accum_add1 in H4. lia.
 } clear IHlsorted.
 destruct H1 as [l1 [l2 [? [? ?]]]].
@@ -1026,7 +1026,7 @@ subst a0. rewrite find_cons. split; intros. apply H5; auto. pose proof (find_lbo
 ****
 subst b. rewrite find_cons. (*falseness*)
 split; intros.
-assert (0 < find (a::l2) a0 0). simpl. destruct (prod_eqdec Z_EqDec Z_EqDec a a0).
+assert (0 < find (a::l2) a0 0). simpl. destruct (E_EqDec a a0).
 hnf in e. subst a0. exfalso; apply Ha. apply in_or_app; right; auto.
 pose proof (find_lbound l2 a0 1). lia.
 lia.
@@ -1039,8 +1039,8 @@ apply H0. left; auto.
 **** rewrite <- H2.
 2: apply in_or_app; right; auto. 2: apply in_or_app; right; auto.
 simpl.
-destruct (prod_eqdec Z_EqDec Z_EqDec a a0). hnf in e; subst a0. exfalso; apply Ha. apply in_or_app; right; auto.
-destruct (prod_eqdec Z_EqDec Z_EqDec a b). hnf in e; subst b. exfalso; apply Ha. apply in_or_app; right; auto.
+destruct (E_EqDec a a0). hnf in e; subst a0. exfalso; apply Ha. apply in_or_app; right; auto.
+destruct (E_EqDec a b). hnf in e; subst b. exfalso; apply Ha. apply in_or_app; right; auto.
 replace 1 with (1+0) by lia. do 2 rewrite find_accum_add1. split; intros; lia.
 Qed.
 
